added more tests

I2SFI/CompilerPBTests.v
@@ -4,6 +4,7 @@
 Require Import Coq.NArith.BinNat.
 Require Import Coq.ZArith.ZArith.
 Require Import Coq.Lists.List.
+Require Import Coq.Strings.String.
 
 Require Import CompCert.Events.
 
@@ -14,67 +15,15 @@ Require Import TargetSFI.Machine.
 Require Import TargetSFI.CS.
 Require Import TargetSFI.EitherMonad.
 Require Import TargetSFI.StateMonad.
+Require Import TargetSFI.MachineGen.
 
 Require Import Intermediate.Machine.
 
 From QuickChick Require Import QuickChick.
 Import QcDefaultNotation. Import QcNotation. Open Scope qc_scope.
 Import GenLow GenHigh.
-
-(* Definition in_memory (start : RiscMachine.address) *)
-(*            (code : list RiscMachine.ISA.instr) *)
-(*            (mem : RiscMachine.Memory.t) : Prop := *)
-(*   fst (List.fold_left *)
-(*          (fun '(p,index) i => *)
-(*             match RiscMachine.Memory.get_instr mem (start + (N.of_nat index))%N with *)
-(*             | Some i' => (p /\ (i = i'),index+1) *)
-(*             | None => (False,index+1) *)
-(*             end) *)
-(*          code (True,0)). *)
-
-(* Definition sfi_registers_correct (regs : RiscMachine.RegisterFile.t) : Prop := True. (* TODO *) *)
-
-(* Definition address_in_same_component (st : MachineState.t) (r : RiscMachine.Register.t) : Prop := *)
-(*   let regs := MachineState.getRegs st in *)
-(*   let pc := MachineState.getPC st in *)
-(*   match RiscMachine.RegisterFile.get_register r regs with *)
-(*   | None => False *)
-(*   | Some v => SFI.is_same_component pc (RiscMachine.Memory.to_address v) *)
-(*   end. *)
-
-Conjecture correct_data_compartmentalized:
-
-  forall (sfi_p : sfi_program) (ip : Intermediate.program)
-    (n : nat) (mem : RiscMachine.Memory.t) (pc : RiscMachine.address)
-    (gen_regs : RiscMachine.RegisterFile.t)
-    (rp rs : RiscMachine.Register.t)
-    (t : CompCert.Events.trace) 
-    (ptr sfi_sp_val: RiscMachine.value ),
-
-    TargetSFI.EitherMonad.Right sfi_p = compile_program ip /\
-    TargetSFI.EitherMonad.Right (t, (mem,pc,gen_regs)) = (CS.eval_program n sfi_p RiscMachine.RegisterFile.reset_all) /\
-    RiscMachine.Memory.get_word mem pc = Some (RiscMachine.Instruction (RiscMachine.ISA.IStore rp rs)) ->
-    (* Write at the top of SFI stack (from a pc that is in the list of push sfi ??) *)
-    (
-      rp = RiscMachine.Register.R_AUX1 /\
-      rs = RiscMachine.Register.R_RA /\
-      Some ptr = RiscMachine.RegisterFile.get_register rp gen_regs /\
-      Some sfi_sp_val = RiscMachine.RegisterFile.get_register
-                          RiscMachine.Register.R_SFI_SP gen_regs /\
-      RiscMachine.Memory.to_address ptr = SFI.address_of SFI.MONITOR_COMPONENT_ID
-                                                  (2*(Z.to_N sfi_sp_val))%N N0 
-    )
-    \/ (* same component write into a data block *)
-    ( Some ptr = RiscMachine.RegisterFile.get_register rp gen_regs /\
-      (Z0 <= ptr)%Z /\    
-      SFI.is_same_component pc (RiscMachine.Memory.to_address ptr) /\
-      (SFI.is_data_address (RiscMachine.Memory.to_address ptr)) = true
-    ).
-
-    
-(************************************************
- * No writes outside it's own memory
- *************************************************)
+(* Suppress some annoying warnings: *)
+Set Warnings "-extraction-opaque-accessed,-extraction".
 
 Instance show_intermediate_program : Show Intermediate.program :=
   {|
@@ -108,7 +57,47 @@ Definition genIntermediateProgram : G Intermediate.program :=
         Intermediate.prog_main := (COMP1_ID,PROC1_ID)
       |}.
 
-Definition store_log := list (RiscMachine.pc * RiscMachine.address * RiscMachine.value).
+
+(* This is how I would like to write the property to test *)
+(* TODO check it later *)
+Conjecture correct_data_compartmentalized:
+
+  forall (sfi_p : sfi_program) (ip : Intermediate.program)
+    (n : nat) (mem : RiscMachine.Memory.t) (pc : RiscMachine.address)
+    (gen_regs : RiscMachine.RegisterFile.t)
+    (rp rs : RiscMachine.Register.t)
+    (t : CompCert.Events.trace) 
+    (ptr sfi_sp_val: RiscMachine.value ),
+
+    TargetSFI.EitherMonad.Right sfi_p = compile_program ip /\
+    TargetSFI.EitherMonad.Right (t, (mem,pc,gen_regs)) = (CS.eval_program n sfi_p RiscMachine.RegisterFile.reset_all) /\
+    RiscMachine.Memory.get_word mem pc = Some (RiscMachine.Instruction (RiscMachine.ISA.IStore rp rs)) ->
+    (* Write at the top of SFI stack (from a pc that is in the list of push sfi ??) *)
+    (
+      rp = RiscMachine.Register.R_AUX1 /\
+      rs = RiscMachine.Register.R_RA /\
+      Some ptr = RiscMachine.RegisterFile.get_register rp gen_regs /\
+      Some sfi_sp_val = RiscMachine.RegisterFile.get_register
+                          RiscMachine.Register.R_SFI_SP gen_regs /\
+      RiscMachine.Memory.to_address ptr = SFI.address_of SFI.MONITOR_COMPONENT_ID
+                                                  (2*(Z.to_N sfi_sp_val))%N N0 
+    )
+    \/ (* same component write into a data block *)
+    ( Some ptr = RiscMachine.RegisterFile.get_register rp gen_regs /\
+      (Z0 <= ptr)%Z /\    
+      SFI.is_same_component pc (RiscMachine.Memory.to_address ptr) /\
+      (SFI.is_data_address (RiscMachine.Memory.to_address ptr)) = true
+    ).
+
+    
+(************************************************
+ * No writes outside it's own memory, 
+ * except for push sfi.
+ *************************************************)
+
+Definition store_log_entry := RiscMachine.pc * RiscMachine.address * RiscMachine.value.
+
+Definition store_log := list store_log_entry.
 
 Definition update_store_log (st : MachineState.t) (t : CompCert.Events.trace)
            (st' : MachineState.t) (log : store_log) :=
@@ -121,7 +110,7 @@ Definition update_store_log (st : MachineState.t) (t : CompCert.Events.trace)
       | Some ptr =>
         let addr := RiscMachine.Memory.to_address ptr in
         match RiscMachine.RegisterFile.get_register RiscMachine.Register.R_SFI_SP regs with
-        | Some sp => log ++ [(pc,addr,sp)]
+        | Some sp => (log ++ [(pc,addr,sp)])%list
         | _ => log
         end
       | _ => log
@@ -131,6 +120,12 @@ Definition update_store_log (st : MachineState.t) (t : CompCert.Events.trace)
   | _ => log
   end.
             
+Definition show_log_entry (entry : store_log_entry) : string :=
+  let '(pc,addr,sfi_sp) := entry in
+   "pc: " ++ (show_addr pc)
+          ++ " ptr: "
+          ++ (show_addr addr)
+          ++ " sfi sp: " ++ (show sfi_sp).
 
 Definition eval_store_program (p : sfi_program)
   : (@Either (CompCert.Events.trace*MachineState.t) * store_log) :=
@@ -141,10 +136,22 @@ Definition eval_store_program (p : sfi_program)
      p
      (RiscMachine.RegisterFile.reset_all)) nil).
   
-Definition store_checker (log : store_log) : Checker := 
-  checker (
-       true (* TODO implement this *)
-    ). 
+Definition store_checker (log : store_log) : Checker :=
+  conjoin (List.map (fun '(pc,addr,sfi_sp) =>
+                       if (SFI.is_same_component_bool pc addr)
+                       then checker true
+                       else
+                         if (N.eqb (SFI.C_SFI addr) SFI.MONITOR_COMPONENT_ID)
+                         then
+                           whenFail ("Failed at: " ++ (show_log_entry (pc,addr,sfi_sp)) )%string
+                                    (N.eqb addr (SFI.address_of
+                                                   SFI.MONITOR_COMPONENT_ID
+                                                   (Z.to_N (2 * sfi_sp +1))
+                                                   0))
+                         else
+                           whenFail ("Failed at: " ++ (show_log_entry (pc,addr,sfi_sp)) )%string
+                                    false
+                    ) log).
 
 Definition store_correct : Checker :=
   forAll genIntermediateProgram
@@ -156,3 +163,216 @@ Definition store_correct : Checker :=
         store_checker log (* check the log even if the program fails *)
       end
   ).
+
+(********************************************
+ * Jumps
+ ************************************************)
+
+Definition jump_log_entry := RiscMachine.pc * RiscMachine.address * CompCert.Events.trace.
+
+Definition jump_log := list (@Either jump_log_entry).
+
+Definition update_jump_log (st : MachineState.t) (t : CompCert.Events.trace)
+           (st' : MachineState.t) (log : jump_log) :=
+  let '(mem,pc,regs) := st in
+  match RiscMachine.Memory.get_word mem pc with
+  | Some (RiscMachine.Instruction instr) =>
+    match instr with
+    | RiscMachine.ISA.IJump r  =>
+      if (N.eqb r RiscMachine.Register.R_RA) || (N.eqb r RiscMachine.Register.R_T)
+      then
+        match RiscMachine.RegisterFile.get_register r regs with
+        | Some ptr => (log ++ [TargetSFI.EitherMonad.Right (pc, RiscMachine.Memory.to_address ptr,t)])%list
+        | _ => log
+        end
+      else
+        (log ++ [TargetSFI.EitherMonad.Left ("Illegal target register: " ++ (show_N r))%string])%list
+    | RiscMachine.ISA.IJal addr => (log ++ [TargetSFI.EitherMonad.Right (pc,addr,t)])%list
+    | _ => log
+    end
+  | Some (RiscMachine.Data _) => (log ++ [TargetSFI.EitherMonad.Left ("Data found at address: " ++ (show pc))%string])%list
+  | _ => log
+  end.
+            
+Definition show_jump_log_entry (entry : jump_log_entry) : string :=
+  let '(pc,addr,t) := entry in
+   "pc: " ++ (show pc)
+          ++ " ptr: "
+          ++ (show addr)
+          ++ " trace: " ++ (show t).
+
+Definition eval_jump_program (p : sfi_program)
+  : (@Either (CompCert.Events.trace*MachineState.t) * jump_log) :=
+  ((CS.eval_program_with_state     
+     jump_log
+     update_jump_log
+     (100%nat)
+     p
+     (RiscMachine.RegisterFile.reset_all)) nil).
+  
+Definition jump_checker (log : jump_log) : Checker :=
+  conjoin (List.map (fun elt =>
+                       match elt with
+                       | TargetSFI.EitherMonad.Left msg => whenFail msg false
+                       | TargetSFI.EitherMonad.Right (pc,addr,t) =>
+                         if (SFI.is_same_component_bool pc addr)
+                            || (N.eqb (SFI.C_SFI addr) SFI.MONITOR_COMPONENT_ID)
+                            || (N.eqb (SFI.C_SFI pc) SFI.MONITOR_COMPONENT_ID)
+                         then
+                           match t with
+                           | nil => checker true
+                           | _ => whenFail ("Unexpectected event at log entry:" ++ (show_jump_log_entry (pc,addr,t)))
+                                          false
+                           end
+                         else
+                           match t with
+                           | _::_ => checker true
+                           | nill => whenFail ("Unexpectected empty event at log entry:" ++ (show_jump_log_entry (pc,addr,t)))
+                                             false
+                           end
+                       end
+                    ) log). (* TODO check the event too *)
+
+Definition jump_correct : Checker :=
+  forAll genIntermediateProgram
+         ( fun ip =>
+             match compile_program ip with
+             | TargetSFI.EitherMonad.Left msg => checker false
+             | TargetSFI.EitherMonad.Right p =>
+               let (res,log) := eval_jump_program p in
+               jump_checker log (* check the log even if the program fails *)
+             end
+         ).
+
+
+(*******************************************************
+ * Control Stack
+ **********************************************************)
+Inductive stack_op := Push
+                    | Pop.
+
+Definition show_op op :=
+  match op with
+  | Push => "Push"
+  | Pop => "Pop"
+  end.
+
+Definition cs_log_entry := RiscMachine.pc * RiscMachine.address * stack_op * RiscMachine.ISA.instr.
+
+Definition cs_log := list (@Either cs_log_entry).
+
+Definition update_cs_log (st : MachineState.t) (t : CompCert.Events.trace)
+           (st' : MachineState.t) (log : cs_log) :=
+  let '(mem,pc,regs) := st in
+  match RiscMachine.Memory.get_word mem pc with
+  | Some (RiscMachine.Instruction instr) =>
+    match instr with
+    | RiscMachine.ISA.IJump r  =>
+        match RiscMachine.RegisterFile.get_register r regs with
+        | Some ptr => let addr := RiscMachine.Memory.to_address ptr in
+                     if SFI.is_same_component_bool pc addr
+                     then (* intra-component jump *)
+                       if (N.eqb r RiscMachine.Register.R_T)
+                       then log
+                       else
+                         (log ++ [TargetSFI.EitherMonad.Left ("Illegal target register: " ++ (show_N r))%string])%list  
+                     else (* cross-component return *)
+                       if (N.eqb r RiscMachine.Register.R_RA)
+                       then
+                         (log ++ [TargetSFI.EitherMonad.Right (pc, addr, Pop, instr)])%list
+                       else
+                         (log ++ [TargetSFI.EitherMonad.Left ("Illegal target register: " ++ (show_N r))%string])%list
+        | _ => (log ++ [TargetSFI.EitherMonad.Left ("Can't find R_RA in general registers " ++ (show regs))%string])%list
+        end
+    | RiscMachine.ISA.IJal addr =>
+      if SFI.is_same_component_bool pc addr
+      then log
+      else
+        let '(mem',pc',regs') := st' in
+        match RiscMachine.RegisterFile.get_register RiscMachine.Register.R_RA regs' with
+        | Some addr => (log ++ [TargetSFI.EitherMonad.Right (pc, RiscMachine.Memory.to_address addr,Push, instr)])%list
+        | _ => (log ++ [TargetSFI.EitherMonad.Left ("Can't find R_RA in general registers " ++ (show regs'))%string])%list
+        end
+    | _ => log
+    end
+  | Some (RiscMachine.Data _) => (log ++ [TargetSFI.EitherMonad.Left ("Data found at address: " ++ (show pc))%string])%list
+  | _ => log
+  end.
+            
+Definition show_cs_log_entry (entry : cs_log_entry) : string :=
+  let '(pc,addr,t, instr) := entry in
+   "pc: " ++ (show_addr pc)
+          ++ " ptr: "
+          ++ (show_addr addr)
+          ++ " stack op: " ++ (show_op t)
+          ++ "instr " ++ (show instr). 
+
+Definition eval_cs_program (p : sfi_program)
+  : (@Either (CompCert.Events.trace*MachineState.t) * cs_log) :=
+  ((CS.eval_program_with_state     
+     cs_log
+     update_cs_log
+     (100%nat)
+     p
+     (RiscMachine.RegisterFile.reset_all)) nil).
+  
+Definition cs_checker (log : cs_log) : Checker :=
+  let fix aux l s :=
+      match l with
+      | nil => checker true
+      | elt::xs =>
+        match elt with
+        | TargetSFI.EitherMonad.Left msg => whenFail msg false
+        | TargetSFI.EitherMonad.Right (pc,addr,op,instr) =>
+          match op with
+          | Push => aux xs (addr::s)
+          | Pop =>
+            match s with
+            | nil => whenFail ("Attemting to pop from empty stack at address" ++ (show pc))%string false
+            | a::s' => if (N.eqb a addr)
+                      then aux xs s'
+                      else whenFail ("Attemting address on the stack: "
+                                       ++ (show_addr a)
+                                       ++ " address in register: "
+                                       ++ (show_addr addr)
+                                       ++ "at pc: "
+                                       ++ (show_addr pc)
+                                       ++ " instr: "
+                                       ++ (show instr)
+                                    )%string
+                                    false
+            end
+          end
+        end
+      end
+  in aux log [].
+
+Definition cs_correct : Checker :=
+  forAll genIntermediateProgram
+         ( fun ip =>
+             match compile_program ip with
+             | TargetSFI.EitherMonad.Left msg => checker false
+             | TargetSFI.EitherMonad.Right p =>
+               let (res,log) := eval_cs_program p in
+               match res with
+               | TargetSFI.EitherMonad.Left msg => whenFail msg (cs_checker log)
+               | TargetSFI.EitherMonad.Right (t,(mem,_,regs)) => 
+                 (whenFail ("memory of failed program: " ++ (show_mem  mem))%string
+                        (cs_checker log) (* check the log even if the program fails *))
+               end
+             end
+         ).
+
+(****************** QUICK CHECKS ***************************)
+QuickChick store_correct.
+QuickChick jump_correct.
+QuickChick cs_correct.
+
+(* test compile correctness *)
+
+(* Conjecture robust_compilation : *)
+(*   forall (ip : Intermediate.program) (sp : sfi_program) *)
+(*     (sc : sfi_program) (b : trace) *)
+
+(*     eval  *)
+(* . *)
